Linkerproof.v
@@ -6,6 +6,7 @@ Require Import Integers Floats Values AST Globalenvs.
 Require Import Errors Behaviors Compiler Smallstep.
 Require Import Language Linker.
 Require Import Tree.
+Require Import LinkerBasicproof.
 
 Require ProgramLSim Adequacy.
 
@@ -20,15 +21,7 @@ Require Deadcodeproof_linker.
 
 Set Implicit Arguments.
 
-(** linker correctness statement *)
-
-Definition linker_correctness :=
-  forall ctree asmtree cprog
-         (CLINK: Tree.reduce (link_program Language_C) ctree = Some cprog)
-         (TRANSF: Tree.Forall2 (fun c a => transf_c_program c = OK a) ctree asmtree),
-  exists (asmprog:Asm.program)
-         (FS:forward_simulation (Cstrategy.semantics cprog) (Asm.semantics asmprog)),
-    Tree.reduce (link_program Language_Asm) asmtree = Some asmprog.
+(** Lemma on applies *)
 
 Lemma apply_partial_inversion:
   forall A B (a:res A) (f:A -> res B) (b:B),
@@ -46,43 +39,6 @@ Proof.
   constructor; intros.
   - destruct H as [? [? ?]]. subst. auto.
   - destruct a; inv H. eexists. split; eauto.
-Qed.
-
-Lemma transform_program_link_program
-      fT1 fT2 vT
-      (tf:(Fundef_common fT1) -> (Fundef_common fT2))
-      (p1 p2 p:(mkLanguage (Fundef_common fT1) vT).(progT))
-      (q1 q2:(mkLanguage (Fundef_common fT2) vT).(progT))
-      (Hp: link_program (mkLanguage (Fundef_common fT1) vT) p1 p2 = Some p)
-      (H1: transform_program tf p1 = q1)
-      (H2: transform_program tf p2 = q2):
-  exists q,
-    link_program (mkLanguage (Fundef_common fT2) vT) q1 q2 = Some q /\
-    transform_program tf p = q.
-Proof.
-  admit.
-Qed.
-
-Lemma transform_partial_program2_link_program
-      (lang_src lang_tgt:Language)
-      (tf:lang_src.(fundefT)->res lang_tgt.(fundefT))
-      (tv:lang_src.(vT)->res lang_tgt.(vT))
-      p1 p2 p q1 q2
-      (Hp: link_program lang_src p1 p2 = Some p)
-      (H1: transform_partial_program2 tf tv p1 = OK q1)
-      (H2: transform_partial_program2 tf tv p2 = OK q2):
-  exists q,
-    link_program lang_tgt q1 q2 = Some q /\
-    transform_partial_program2 tf tv p = OK q.
-Proof.
-  destruct p1 as [p1 mainp1], p2 as [p2 mainp2], q1 as [q1 mainq1], q2 as [q2 mainq2].
-  rewrite transform_partial_program2_augment in *. simpl in *.
-  apply transform_partial_augment_program_match in H1. destruct H1 as [[qdefs1 [Hqdefs1 ?]] Hmain1].
-  apply transform_partial_augment_program_match in H2. destruct H2 as [[qdefs2 [Hqdefs2 ?]] Hmain2].
-  simpl in *. rewrite app_nil_r in *. symmetry in H, H0. subst.
-  unfold link_program in *. simpl in *. destruct (Pos.eqb mainp1 mainp2) eqn:Hmainp; [|inv Hp].
-  apply Peqb_true_eq in Hmainp. subst.
-  admit.
 Qed.
 
 Ltac clarify :=
