common/LinkerBasicproof.v
@@ -1,0 +1,197 @@
+Require Import RelationClasses.
+Require String.
+Require Import Coqlib Coqlib_linker.
+Require Import Maps Maps_linker.
+Require Import Integers Floats Values AST Globalenvs.
+Require Import Errors Behaviors Compiler Smallstep.
+Require Import Language Linker LinkerProp.
+
+(** lemma on link_globdefs *)
+
+Lemma link_globdefs_morphism
+      lang p1 p2 p p1' p2'
+      (H: link_globdefs lang p1 p2 = Some p)
+      (H1: PTree_eq p1 p1') (H2: PTree_eq p2 p2'):
+  exists p',
+    link_globdefs lang p1' p2' = Some p' /\
+    PTree_eq p p'.
+Proof.
+  admit.
+Qed.
+
+(** Lemma on transform_program_globdef *)
+
+Lemma find_map_transform_program_globdef A B V (tf:A->B) (p:list (ident * globdef A V)) i:
+  find
+    (fun id : positive * globdef B V => peq i (fst id))
+    (map (transform_program_globdef tf) p) =
+  option_map
+    (transform_program_globdef tf)
+    (find (fun id : positive * globdef A V => peq i (fst id)) p).
+Proof.
+  induction p; simpl; auto.
+  unfold transform_program_globdef in *. destruct a. destruct g; simpl.
+  - destruct (peq i i0); subst; simpl; auto.
+  - destruct (peq i i0); subst; simpl; auto.
+Qed.
+
+Lemma option_map_snd_transform_program_globdef A B V (tf:A->B) (g:option (ident * globdef A V)):
+  option_map snd (option_map (transform_program_globdef tf) g) =
+  match option_map snd g with
+    | Some (Gfun f) => Some (Gfun (tf f))
+    | Some (Gvar v) => Some (Gvar v)
+    | None => None
+  end.
+Proof. destruct g; auto. destruct p. destruct g; auto. Qed.
+
+Lemma PTree_unelements_map_transform_program_globdef A B V (tf:A->B) (p:list (ident * globdef A V)):
+  PTree_eq
+    (PTree_unelements (map (transform_program_globdef tf) p))
+    (PTree.map
+       (fun i g =>
+          match g with
+            | Gfun f => Gfun (tf f)
+            | Gvar v => Gvar v
+          end)
+       (PTree_unelements p)).
+Proof.
+  unfold PTree_unelements. rewrite <- ? fold_left_rev_right.
+  rewrite <- map_rev. unfold ident in *. simpl in *.
+  induction (rev p); simpl.
+  { constructor. intros. rewrite PTree.gmap, ? PTree.gempty. auto. }
+  inv IHl. constructor. intros. specialize (H i).
+  rewrite ? PTree.gmap, ? PTree.gsspec in *. destruct a. destruct g; simpl.
+  - destruct (peq i p0); auto.
+  - destruct (peq i p0); auto.
+Qed.
+
+Lemma map_transform_program_globdef_PTree_elements A B V (tf:A->B) (p:PTree.t (globdef A V)):
+  map (transform_program_globdef tf) (PTree.elements p) =
+  PTree.elements
+    (PTree.map
+       (fun i g =>
+          match g with
+            | Gfun f => Gfun (tf f)
+            | Gvar v => Gvar v
+          end)
+       p).
+Proof.
+  exploit (PTree.elements_canonical_order
+             (fun g1 g2 => g2 =
+                           match g1 with
+                             | Gfun f => Gfun (tf f)
+                             | Gvar v => Gvar v
+                           end)
+             p
+             (PTree.map
+                (fun (_ : positive) (g : globdef A V) =>
+                   match g with
+                     | Gfun f => Gfun (tf f)
+                     | Gvar v => Gvar v
+                   end) p)).
+  - intros. eexists. split; auto. rewrite PTree.gmap, H. auto.
+  - intros. rewrite PTree.gmap in H. destruct (p ! i) eqn:Hpi; inv H. eexists. split; auto.
+  - generalize ((PTree.elements
+                   (PTree.map
+                      (fun (_ : positive) (g : globdef A V) =>
+                         match g with
+                           | Gfun f => Gfun (tf f)
+                           | Gvar v => Gvar v
+                         end) p))).
+    generalize (PTree.elements p). clear p.
+    induction l; intros l0 X; inv X; auto.
+    destruct a, b1, H1 as [? ?]. simpl in *. subst.
+    f_equal; auto. destruct g; auto.
+Qed.
+
+(** lemma on transform_program *)
+
+Lemma transform_program_link_program
+      (fT1 fT2:F Sig_signature) vT
+      (tf:fT1 -> fT2)
+      (p1 p2 p:(mkLanguage (Fundef_common fT1) vT).(progT))
+      (q1 q2:(mkLanguage (Fundef_common fT2) vT).(progT))
+      (Hp: link_program (mkLanguage (Fundef_common fT1) vT) p1 p2 = Some p)
+      (H1: transform_program (AST.transf_fundef tf) p1 = q1)
+      (H2: transform_program (AST.transf_fundef tf) p2 = q2):
+  exists q,
+    link_program (mkLanguage (Fundef_common fT2) vT) q1 q2 = Some q /\
+    transform_program (AST.transf_fundef tf) p = q.
+Proof.
+  Ltac clarify :=
+    repeat match goal with
+             | [H: context[match ?d with | Some _ => _ | None => _ end] |- _] =>
+               let defs := fresh "defs" in
+               let Hdefs := fresh "Hdefs" in
+               destruct d as [defs|] eqn:Hdefs; inv H; simpl in *
+             | [|- context[match ?d with | Some _ => _ | None => _ end]] =>
+               let defs := fresh "defs" in
+               let Hdefs := fresh "Hdefs" in
+               destruct d as [defs|] eqn:Hdefs; simpl in *
+           end.
+  unfold progT in *. simpl in *. subst.
+  unfold link_program, transform_program in *. simpl in *.
+  destruct p1 as [p1 mainp1], p2 as [p2 mainp2]. simpl in *.
+  destruct (Pos.eqb mainp1 mainp2); [|inv Hp]. clarify.
+  - unfold link_globdef_list in *. clarify.
+    eexists. split; eauto. repeat f_equal.
+    eapply (link_globdefs_morphism (mkLanguage (Fundef_common fT2) vT)) in Hdefs1;
+      try apply PTree_unelements_map_transform_program_globdef. simpl in *.
+    destruct Hdefs1 as [defs1' [Hdefs1' Hdefs1]]. rewrite (PTree_elements_extensional' Hdefs1).
+    clear defs1 Hdefs1.
+    revert Hdefs0 Hdefs1'. generalize (PTree_unelements p1) (PTree_unelements p2).
+    clear p1 p2. intros p1 p2 Hdefs0 Hdefs1'.
+    rewrite map_transform_program_globdef_PTree_elements.
+    apply PTree_elements_extensional'. constructor. intro. rewrite PTree.gmap.
+    eapply (gtlink_globdefs (mkLanguage (Fundef_common fT1) vT)) in Hdefs0. instantiate (1 := i) in Hdefs0.
+    eapply (gtlink_globdefs (mkLanguage (Fundef_common fT2) vT)) in Hdefs1'. instantiate (1 := i) in Hdefs1'.
+    rewrite PTree.gmap in *. unfold ident in *. simpl in *.
+    destruct (p1 ! i); simpl in *; rewrite PTree.gmap in *;
+    destruct (p2 ! i), (defs0 ! i), (defs1' ! i); simpl in *; subst; auto;
+    try match goal with
+          | [H: False |- _] => inv H
+        end.
+    destruct Hdefs0 as [[? ?]|[? ?]], Hdefs1' as [[? ?]|[? ?]]; subst; auto.
+    + admit.
+    + admit.
+  - exfalso. unfold link_globdef_list in *. clarify.
+    eapply (gflink_globdefs (mkLanguage (Fundef_common fT2) vT)) in Hdefs1. simpl in *.
+    destruct Hdefs1 as [i [tdef1 [tdef2 [Htdef1 [Htdef2 [Htdefs1 Htdefs2]]]]]].
+    eapply (gtlink_globdefs (mkLanguage (Fundef_common fT1) vT)) in Hdefs0. instantiate (1 := i) in Hdefs0. simpl in *.
+    rewrite PTree_guespec in Htdef1. rewrite PTree_guespec in Htdef2.
+    rewrite <- map_rev in *. rewrite ? PTree_guespec in Hdefs0.
+    rewrite find_map_transform_program_globdef in *.
+    rewrite option_map_snd_transform_program_globdef in *.
+    clarify.
+    unfold ident in *. rewrite Hdefs, Hdefs1 in Hdefs0. clarify.
+    + destruct H as [H ?]. subst.
+      contradict Htdefs1. inv H.
+      * inv H0. inv H1. constructor. admit.
+      * inv H0. inv H1. constructor. inv Hv. constructor; auto.
+    + destruct H as [H ?]. subst.
+      contradict Htdefs2. inv H.
+      * inv H0. inv H1. constructor. admit.
+      * inv H0. inv H1. constructor. inv Hv. constructor; auto.
+Qed.
+
+Lemma transform_partial_program2_link_program
+      (lang_src lang_tgt:Language)
+      (tf:lang_src.(fundefT)->res lang_tgt.(fundefT))
+      (tv:lang_src.(vT)->res lang_tgt.(vT))
+      p1 p2 p q1 q2
+      (Hp: link_program lang_src p1 p2 = Some p)
+      (H1: transform_partial_program2 tf tv p1 = OK q1)
+      (H2: transform_partial_program2 tf tv p2 = OK q2):
+  exists q,
+    link_program lang_tgt q1 q2 = Some q /\
+    transform_partial_program2 tf tv p = OK q.
+Proof.
+  destruct p1 as [p1 mainp1], p2 as [p2 mainp2], q1 as [q1 mainq1], q2 as [q2 mainq2].
+  rewrite transform_partial_program2_augment in *. simpl in *.
+  apply transform_partial_augment_program_match in H1. destruct H1 as [[qdefs1 [Hqdefs1 ?]] Hmain1].
+  apply transform_partial_augment_program_match in H2. destruct H2 as [[qdefs2 [Hqdefs2 ?]] Hmain2].
+  simpl in *. rewrite app_nil_r in *. symmetry in H, H0. subst.
+  unfold link_program in *. simpl in *. destruct (Pos.eqb mainp1 mainp2) eqn:Hmainp; [|inv Hp].
+  apply Peqb_true_eq in Hmainp. subst.
+  admit.
+Qed.
